feat: Polymorph materials (#405)

src/AwsCryptographicMaterialProviders/AlgorithmSuites.dfy
@@ -3,6 +3,7 @@
 
 include "../StandardLibrary/StandardLibrary.dfy"
 include "../Generated/AwsCryptographicMaterialProviders.dfy"
+include "../../libraries/src/Collections/Maps/Maps.dfy"
 
 module 
   {:extern "Dafny.Aws.Crypto.AwsCryptographicMaterialProvidersClient2.AlgorithmSuites"}
@@ -11,6 +12,7 @@ module
   import opened Wrappers
   import opened StandardLibrary
   import opened UInt = StandardLibrary.UInt
+  import Maps
   import Aws.Crypto
 
   type KeyLength = l: uint8 | l == 32 || l == 24 || l == 16 witness 32
@@ -189,4 +191,27 @@ module
     commitment := CommitmentDerivationAlgorithm.Algorithm(KeyDerivationAlgorithm_.HKDF_WITH_SHA_512(Bits256, Bits256)),
     signature := SignatureAlgorithm.ECDSA_P_384_SHA_384
   )
+
+  const SupportedAlgorithmSuites: map<Crypto.AlgorithmSuiteId, AlgorithmSuite> := map[
+    Crypto.AlgorithmSuiteId.ALG_AES_128_GCM_IV12_TAG16_NO_KDF := ALG_AES_128_GCM_IV12_TAG16_NO_KDF,
+    Crypto.AlgorithmSuiteId.ALG_AES_192_GCM_IV12_TAG16_NO_KDF := ALG_AES_192_GCM_IV12_TAG16_NO_KDF,
+    Crypto.AlgorithmSuiteId.ALG_AES_256_GCM_IV12_TAG16_NO_KDF := ALG_AES_256_GCM_IV12_TAG16_NO_KDF,
+    Crypto.AlgorithmSuiteId.ALG_AES_128_GCM_IV12_TAG16_HKDF_SHA256 := ALG_AES_128_GCM_IV12_TAG16_HKDF_SHA256,
+    Crypto.AlgorithmSuiteId.ALG_AES_192_GCM_IV12_TAG16_HKDF_SHA256 := ALG_AES_192_GCM_IV12_TAG16_HKDF_SHA256,
+    Crypto.AlgorithmSuiteId.ALG_AES_256_GCM_IV12_TAG16_HKDF_SHA256 := ALG_AES_256_GCM_IV12_TAG16_HKDF_SHA256,
+    Crypto.AlgorithmSuiteId.ALG_AES_128_GCM_IV12_TAG16_HKDF_SHA256_ECDSA_P256 := ALG_AES_128_GCM_IV12_TAG16_HKDF_SHA256_ECDSA_P256,
+    Crypto.AlgorithmSuiteId.ALG_AES_192_GCM_IV12_TAG16_HKDF_SHA384_ECDSA_P384 := ALG_AES_192_GCM_IV12_TAG16_HKDF_SHA384_ECDSA_P384,
+    Crypto.AlgorithmSuiteId.ALG_AES_256_GCM_IV12_TAG16_HKDF_SHA384_ECDSA_P384 := ALG_AES_256_GCM_IV12_TAG16_HKDF_SHA384_ECDSA_P384,
+    Crypto.AlgorithmSuiteId.ALG_AES_256_GCM_HKDF_SHA512_COMMIT_KEY := ALG_AES_256_GCM_HKDF_SHA512_COMMIT_KEY,
+    Crypto.AlgorithmSuiteId.ALG_AES_256_GCM_HKDF_SHA512_COMMIT_KEY_ECDSA_P384 := ALG_AES_256_GCM_HKDF_SHA512_COMMIT_KEY_ECDSA_P384
+  ];
+
+  lemma LemmaSupportedAlgorithmSuitesIsComplete(id:Crypto.AlgorithmSuiteId)
+    ensures id in SupportedAlgorithmSuites
+  {}
+
+  function method GetSuite(id: Crypto.AlgorithmSuiteId): (res: AlgorithmSuite) {
+    LemmaSupportedAlgorithmSuitesIsComplete(id);
+    SupportedAlgorithmSuites[id]
+  }
 }
