src/AwsCryptographicMaterialProviders/Materials.dfy
@@ -1,0 +1,183 @@
+// Copyright Amazon.com Inc. or its affiliates. All Rights Reserved.
+// SPDX-License-Identifier: Apache-2.0
+
+include "../StandardLibrary/StandardLibrary.dfy"
+include "../Generated/AwsCryptographicMaterialProviders.dfy" 
+include "AlgorithmSuites.dfy"
+
+module 
+  {:extern "Dafny.Aws.Crypto.AwsCryptographicMaterialProvidersClient2.Materials"}
+  AwsCryptographicMaterialProviders2.Materials
+{
+import opened StandardLibrary
+  import opened Wrappers
+  import opened UInt = StandardLibrary.UInt
+  import UTF8
+  import Aws.Crypto
+  import AlgorithmSuites
+
+  // UTF-8 encoded "aws-crypto-public-key"
+  const EC_PUBLIC_KEY_FIELD: UTF8.ValidUTF8Bytes :=
+    var s :=
+      [0x61, 0x77, 0x73, 0x2D, 0x63, 0x72, 0x79, 0x70, 0x74, 0x6F, 0x2D, 0x70,
+      0x75, 0x62, 0x6C, 0x69, 0x63, 0x2D, 0x6B, 0x65, 0x79];
+    assert UTF8.ValidUTF8Range(s, 0, 21);
+    s
+  const RESERVED_KEY_VALUES := { EC_PUBLIC_KEY_FIELD }
+
+
+  // Encryption Materials
+
+  /* The goal of EncryptionMaterialsTransitionIsValid is to aproxomate
+   * _some_ mutablity in an otherwise immutable structure.
+   * Encryption Materials should allow for the addition
+   * of the plaintext data key and encrypted data keys.
+   * Once a plaintext data key is added,
+   * it can never be removed or altered.
+   * Simmilarly encrypted data keys can be added,
+   * but none can be removed.
+   * This lets keyrings/CMM handle immutalbe data,
+   * and easily assert these invariants.
+   */
+  predicate method EncryptionMaterialsTransitionIsValid(
+    oldMat: Crypto.EncryptionMaterials,
+    newMat: Crypto.EncryptionMaterials
+  ) {
+    && newMat.algorithmSuiteId == oldMat.algorithmSuiteId
+    && newMat.encryptionContext == oldMat.encryptionContext
+    && newMat.signingKey == oldMat.signingKey
+    && (oldMat.plaintextDataKey.None? || oldMat.plaintextDataKey == newMat.plaintextDataKey)
+    && |newMat.encryptedDataKeys| >= |oldMat.encryptedDataKeys|
+    && multiset(oldMat.encryptedDataKeys) <= multiset(newMat.encryptedDataKeys)
+    && ValidEncryptionMaterials(oldMat)
+    && ValidEncryptionMaterials(newMat)
+  }
+
+  predicate method ValidEncryptionMaterials(encryptionMaterials: Crypto.EncryptionMaterials) {
+    && var suite := AlgorithmSuites.GetSuite(encryptionMaterials.algorithmSuiteId);
+    && (suite.signature.None? <==> encryptionMaterials.signingKey.None?)
+    && (encryptionMaterials.plaintextDataKey.Some? ==> suite.keyLen as int == |encryptionMaterials.plaintextDataKey.value|)
+    && (encryptionMaterials.plaintextDataKey.None? ==> |encryptionMaterials.encryptedDataKeys| == 0)
+  }
+
+  function method EncryptionMaterialAddEncryptedDataKeys(
+    encryptionMaterials: Crypto.EncryptionMaterials,
+    encryptedDataKeys: Crypto.EncryptedDataKeyList
+  )
+    :(res: Result<Crypto.EncryptionMaterials, string>)
+    ensures res.Success?
+    ==>
+      && res.value.plaintextDataKey.Some?
+      && EncryptionMaterialsTransitionIsValid(encryptionMaterials, res.value)
+  {
+    :- Need(ValidEncryptionMaterials(encryptionMaterials), "Attempt to modifiy invalid encryption material.");
+    :- Need(encryptionMaterials.plaintextDataKey.Some?, "Adding encrypted data keys without a plaintext data key is not allowed.");
+    Success(Crypto.EncryptionMaterials(
+      plaintextDataKey := encryptionMaterials.plaintextDataKey,
+      encryptedDataKeys := encryptionMaterials.encryptedDataKeys + encryptedDataKeys,
+      algorithmSuiteId := encryptionMaterials.algorithmSuiteId,
+      encryptionContext := encryptionMaterials.encryptionContext,
+      signingKey := encryptionMaterials.signingKey
+    ))
+  }
+
+  function method EncryptionMaterialAddDataKey(
+    encryptionMaterials: Crypto.EncryptionMaterials,
+    plaintextDataKey: seq<uint8>,
+    encryptedDataKeys: Crypto.EncryptedDataKeyList
+  )
+    :(res: Result<Crypto.EncryptionMaterials, string>)
+    ensures res.Success?
+    ==>
+      && res.value.plaintextDataKey.Some?
+      && EncryptionMaterialsTransitionIsValid(encryptionMaterials, res.value)
+  {
+    var suite := AlgorithmSuites.GetSuite(encryptionMaterials.algorithmSuiteId);
+    :- Need(ValidEncryptionMaterials(encryptionMaterials), "Attempt to modifiy invalid encryption material.");
+    :- Need(encryptionMaterials.plaintextDataKey.None?, "Attempt to modify plaintextDataKey.");
+    :- Need(suite.keyLen as int == |plaintextDataKey|, "plaintextDataKey does not match Algorithm Suite specification.");
+
+    Success(Crypto.EncryptionMaterials(
+      plaintextDataKey := Some(plaintextDataKey),
+      encryptedDataKeys := encryptionMaterials.encryptedDataKeys + encryptedDataKeys,
+      algorithmSuiteId := encryptionMaterials.algorithmSuiteId,
+      encryptionContext := encryptionMaterials.encryptionContext,
+      signingKey := encryptionMaterials.signingKey
+    ))
+  }
+
+  // Decryption Materials
+  /* The goal of DecryptionMaterialsTransitionIsValid is to aproxomate
+   * _some_ mutablity in an otherwise immutable structure.
+   * Decryption Materials allow for the addition
+   * of a plaintext data key.
+   * Once a plaintext data key is added,
+   * it can never be removed or altered.
+   * This lets keyrings/CMM handle immutalbe data,
+   * and easily assert these invariants.
+   */
+  predicate method DecryptionMaterialsTransitionIsValid(
+    oldMat: Crypto.DecryptionMaterials,
+    newMat: Crypto.DecryptionMaterials
+  ) {
+    && newMat.algorithmSuiteId == oldMat.algorithmSuiteId
+    && newMat.encryptionContext == oldMat.encryptionContext
+    && newMat.verificationKey == oldMat.verificationKey
+    && (oldMat.plaintextDataKey.None? || oldMat.plaintextDataKey == newMat.plaintextDataKey)
+    && ValidDecryptionMaterials(oldMat)
+    && ValidDecryptionMaterials(newMat)
+  }
+
+  predicate method ValidDecryptionMaterials(decryptionMaterials: Crypto.DecryptionMaterials) {
+    && var suite := AlgorithmSuites.GetSuite(decryptionMaterials.algorithmSuiteId);
+    && (decryptionMaterials.plaintextDataKey.Some? ==> suite.keyLen as int == |decryptionMaterials.plaintextDataKey.value|)
+    && (suite.signature.None? <==> decryptionMaterials.verificationKey.None?)
+  }
+
+  function method DecryptionMaterialsAddDataKey(
+    decryptionMaterials: Crypto.DecryptionMaterials,
+    plaintextDataKey: seq<uint8>
+  )
+    :(res: Result<Crypto.DecryptionMaterials, string>)
+    ensures res.Success?
+    ==>
+      && res.value.plaintextDataKey.Some?
+      && DecryptionMaterialsTransitionIsValid(decryptionMaterials, res.value)
+  {
+    var suite := AlgorithmSuites.GetSuite(decryptionMaterials.algorithmSuiteId);
+    :- Need(ValidDecryptionMaterials(decryptionMaterials), "Attempt to modifiy invalid decryption material.");
+    :- Need(decryptionMaterials.plaintextDataKey.None?, "Attempt to modify plaintextDataKey.");
+    :- Need(suite.keyLen as int == |plaintextDataKey|, "plaintextDataKey does not match Algorithm Suite specification.");
+
+    Success(Crypto.DecryptionMaterials(
+      plaintextDataKey := Some(plaintextDataKey),
+      algorithmSuiteId := decryptionMaterials.algorithmSuiteId,
+      encryptionContext := decryptionMaterials.encryptionContext,
+      verificationKey := decryptionMaterials.verificationKey
+    ))
+  }
+
+  predicate method DecryptionMaterialsWithoutPlaintextDataKey(decryptionMaterials: Crypto.DecryptionMaterials) {
+    && decryptionMaterials.plaintextDataKey.None?
+    && ValidDecryptionMaterials(decryptionMaterials)
+  }
+
+  predicate method DecryptionMaterialsWithPlaintextDataKey(decryptionMaterials: Crypto.DecryptionMaterials) {
+    && decryptionMaterials.plaintextDataKey.Some?
+    && ValidDecryptionMaterials(decryptionMaterials)
+  }
+
+  // The distiction between DecryptionMaterials with and without a PlaintextDataKey
+  // is relevant to DecryptionMaterials in a way that it is not for EncryptionMaterials.
+  // To avoid ambuguity a keyring that recives DecryptionMaterials with a PlaintextDataKey MUST fail.
+  // Given the failure mode of the MultiKeyring,
+  // or any other rational compinator.
+  type DecryptionMaterialsPendingPlaintextDataKey = d: Crypto.DecryptionMaterials
+    | DecryptionMaterialsWithoutPlaintextDataKey(d)
+    witness *
+
+  type SealedDecryptionMaterials = d: Crypto.DecryptionMaterials
+    | DecryptionMaterialsWithPlaintextDataKey(d)
+    witness *
+
+}
